src/Iris/Instances/IProp/Instance.lean
@@ -70,13 +70,11 @@ theorem IProp.unfoldi_foldi (x : FF.api τ (IPre FF)) : unfoldi (foldi x) ≡ x 
   refine .trans (OFunctor.map_comp (F := FF τ |>.fst) ..).symm ?_
   refine .trans ?_ (OFunctor.map_id (F := FF τ |>.fst) x)
   apply OFunctor.map_ne.eqv <;> intro _ <;> simp [IProp.unfold, IProp.fold]
-  all_goals sorry
 
 theorem IProp.proj_fold_unfold (x : FF.api τ (IProp FF)) : foldi (unfoldi x) ≡ x := by
   refine .trans (OFunctor.map_comp (F := FF τ |>.fst) ..).symm ?_
   refine .trans ?_ (OFunctor.map_id (F := FF τ |>.fst) x)
   apply OFunctor.map_ne.eqv <;> intro _ <;> simp [IProp.unfold, IProp.fold]
-  all_goals sorry
 
 end Fold
 
@@ -85,10 +83,10 @@ section iSingleton
 open IProp OFE UPred
 
 def iSingleton {GF} F [RFunctorContractive F] [E : ElemG GF F] (γ : GName) (v : F.ap (IProp GF)) : IResUR GF :=
-  fun τ' γ' =>
+  fun τ' => ⟨fun γ' =>
     if H : (τ' = E.τ ∧ γ' = γ)
       then some (H.1 ▸ (unfoldi <| E.Bundle v))
-      else none
+      else none⟩
 
 theorem IResUR_op_eval {GF} (c1 c2 : IResUR GF) : (c1 • c2) τ' γ' = (c1 τ' γ') • (c2 τ' γ') := by
     simp [CMRA.op, optionOp]
@@ -112,7 +110,7 @@ theorem iSingleton_op {γ : GName} [RFunctorContractive F] [E : ElemG GF F]
   simp [optionOp]
   rename_i h; rcases h with ⟨h1, h2⟩; subst h1; subst h2; simp
   simp [IProp.unfoldi]
-  -- Not sure, but I believe it
+  -- I believe it
   sorry
 
 end iSingleton
@@ -141,6 +139,7 @@ theorem iOwn_mono {a1 a2 : F.ap (IProp GF)} (H : a2 ≼ a1) : iOwn γ a1 ⊢ iOw
   refine .trans ?_ CMRA.op_assocN.symm
   rw [IResUR_op_eval]
   unfold iSingleton
+  simp
   split
   · refine Dist.op_l ?_
     simp [CMRA.op, optionOp]
@@ -152,10 +151,12 @@ theorem iOwn_mono {a1 a2 : F.ap (IProp GF)} (H : a2 ≼ a1) : iOwn γ a1 ⊢ iOw
 theorem iOwn_cmraValid {a : F.ap (IProp GF)} : iOwn γ a ⊢ UPred.cmraValid a := by
   refine .trans (UPred.ownM_valid _) ?_
   refine UPred.valid_entails (fun n H => ?_)
-  specialize H E.τ γ
-  simp [iSingleton, CMRA.ValidN, optionValidN] at H
-  -- Should hold
+  specialize H E.τ
   sorry
+  -- specialize H γ
+  -- simp [iSingleton, CMRA.ValidN, optionValidN] at H
+  -- -- Should hold
+  -- sorry
 
 theorem iOwn_cmraValid_op {a1 a2 : F.ap (IProp GF)} : iOwn γ a1 ∗ iOwn γ a2 ⊢ UPred.cmraValid (a1 • a2) :=
   iOwn_op.mpr.trans iOwn_cmraValid
@@ -175,6 +176,163 @@ instance {a : F.ap (IProp GF)} [CMRA.CoreId a] : BI.Persistent (iOwn γ a) where
     refine OFE.NonExpansive.eqv ?_
     -- Core is element-wise, then use CoreId inst
     sorry
+
+
+theorem iOwn_alloc_strong_dep {f : GName → F.ap (IProp GF)} {P : GName → Prop}
+    (HI : Infinite P) (Hv : ∀ γ, P γ → ✓ (f γ)) :
+    ⊢ |==> ∃ γ, ⌜P γ⌝ ∗ iOwn γ (f γ) := by
+  refine .trans (Q := iprop(|==> ∃ m : IResUR GF, ⌜∃ γ, P γ ∧ m = iSingleton _ γ (f γ)⌝ ∧ UPred.ownM m)) ?_ ?_
+  · refine .trans (UPred.ownM_unit _) <| BI.intuitionistically_elim.trans ?_
+    refine UPred.ownM_updateP _ (fun n mz Hv => ?_)
+    rcases HI with ⟨PE, HPE⟩
+    refine ⟨iSingleton F (PE 0) (f (PE 0)), ⟨_, HPE.inc, rfl⟩, ?_⟩
+    refine fun γ => ⟨fun γ' => ?_, ?_⟩
+    · simp [CMRA.ValidN, optionValidN, CMRA.op?]
+      rcases mz with (_|z) <;> simp only []
+      · simp [iSingleton]
+        rcases Classical.em (γ = ElemG.τ GF F ∧ γ' = PE 0) with (h | h)
+        · simp_all
+          -- By specialization of Hv, getting P from the Enum, and casting
+          sorry
+        · simp_all only [↓reduceDIte]
+      · simp [CMRA.op, optionOp]
+        -- ?
+        sorry
+    · exists (Poke PE 0)
+      -- Remove the 0th term from the enum, it is still infinite
+      sorry
+  · refine BIUpdate.mono ?_
+    refine BI.exists_elim (fun m => ?_)
+    refine BI.pure_elim (φ := ∃ γ, P γ ∧ m = iSingleton F γ (f γ)) BI.and_elim_l ?_
+    refine fun ⟨γ, HP, Hm⟩ => BI.and_elim_r' ?_
+    refine BI.exists_intro' γ ?_
+    refine BI.emp_sep.mpr.trans (BI.sep_mono ?_ ?_)
+    · exact BI.pure_intro HP
+    · rw [Hm]; exact .rfl
+
+theorem iOwn_alloc_dep (f : GName → F.ap (IProp GF)) (Ha : ∀ γ, ✓ (f γ)) :
+    ⊢ |==> ∃ γ, iOwn γ (f γ) :=
+  (iOwn_alloc_strong_dep .Nat_True (fun _ => Ha ·)).trans <|
+  BIUpdate.mono <| BI.exists_mono fun _ => BI.sep_elim_r
+
+theorem iOwn_alloc (a : F.ap (IProp GF)) : ✓ a → ⊢ |==> ∃ γ, iOwn γ a :=
+  fun Ha => iOwn_alloc_dep _ (fun _ => Ha)
+
+theorem iOwn_updateP P γ a : a ~~>: P → iOwn γ a ⊢ |==> ∃ a' : F.ap (IProp GF), ⌜P a'⌝ ∗ iOwn γ a' :=
+  sorry
+
+theorem iOwn_update γ (a a' : F.ap (IProp GF)) : a ~~> a' → iOwn γ a ⊢ |==> iOwn γ a' :=
+  sorry
+
+
+
+/-
+(** ** Allocation *)
+(* TODO: This also holds if we just have ✓ a at the current step-idx, as Iris
+   assertion. However, the map_updateP_alloc does not suffice to show this. *)
+Lemma own_alloc_strong_dep (f : gname → A) (P : gname → Prop) :
+  pred_infinite P →
+  (∀ γ, P γ → ✓ (f γ)) →
+  ⊢ |==> ∃ γ, ⌜P γ⌝ ∗ own γ (f γ).
+Proof.
+  intros HPinf Hf.
+  rewrite -(bupd_mono (∃ m, ⌜∃ γ, P γ ∧ m = iRes_singleton γ (f γ)⌝ ∧ uPred_ownM m)%I).
+  - rewrite /bi_emp_valid (ownM_unit emp).
+    apply bupd_ownM_updateP, (discrete_fun_singleton_updateP_empty _ (λ m, ∃ γ,
+      m = {[ γ := inG_unfold (cmra_transport inG_prf (f γ)) ]} ∧ P γ));
+      [|naive_solver].
+    apply (alloc_updateP_strong_dep _ P _ (λ γ,
+      inG_unfold (cmra_transport inG_prf (f γ)))); [done| |naive_solver].
+    intros γ _ ?.
+    by apply (cmra_morphism_valid inG_unfold), cmra_transport_valid, Hf.
+  - apply exist_elim=>m; apply pure_elim_l=>-[γ [Hfresh ->]].
+    by rewrite !own_eq /own_def -(exist_intro γ) pure_True // left_id.
+Qed.
+Lemma own_alloc_cofinite_dep (f : gname → A) (G : gset gname) :
+  (∀ γ, γ ∉ G → ✓ (f γ)) → ⊢ |==> ∃ γ, ⌜γ ∉ G⌝ ∗ own γ (f γ).
+Proof.
+  intros Ha.
+  apply (own_alloc_strong_dep f (λ γ, γ ∉ G))=> //.
+  apply (pred_infinite_set (C:=gset gname)).
+  intros E. set (γ := fresh (G ∪ E)).
+  exists γ. apply not_elem_of_union, is_fresh.
+Qed.
+Lemma own_alloc_dep (f : gname → A) :
+  (∀ γ, ✓ (f γ)) → ⊢ |==> ∃ γ, own γ (f γ).
+Proof.
+  intros Ha. rewrite /bi_emp_valid (own_alloc_cofinite_dep f ∅) //; [].
+  apply bupd_mono, exist_mono=>?. apply: sep_elim_r.
+Qed.
+
+Lemma own_alloc_strong a (P : gname → Prop) :
+  pred_infinite P →
+  ✓ a → ⊢ |==> ∃ γ, ⌜P γ⌝ ∗ own γ a.
+Proof. intros HP Ha. eapply (own_alloc_strong_dep (λ _, a)); eauto. Qed.
+Lemma own_alloc_cofinite a (G : gset gname) :
+  ✓ a → ⊢ |==> ∃ γ, ⌜γ ∉ G⌝ ∗ own γ a.
+Proof. intros Ha. eapply (own_alloc_cofinite_dep (λ _, a)); eauto. Qed.
+Lemma own_alloc a : ✓ a → ⊢ |==> ∃ γ, own γ a.
+Proof. intros Ha. eapply (own_alloc_dep (λ _, a)); eauto. Qed.
+
+(** ** Frame preserving updates *)
+Lemma own_updateP P γ a : a ~~>: P → own γ a ⊢ |==> ∃ a', ⌜P a'⌝ ∗ own γ a'.
+Proof.
+  intros Hupd. rewrite !own_eq.
+  rewrite -(bupd_mono (∃ m,
+    ⌜ ∃ a', m = iRes_singleton γ a' ∧ P a' ⌝ ∧ uPred_ownM m)%I).
+  - apply bupd_ownM_updateP, (discrete_fun_singleton_updateP _ (λ m, ∃ x,
+      m = {[ γ := x ]} ∧ ∃ x',
+      x = inG_unfold x' ∧ ∃ a',
+      x' = cmra_transport inG_prf a' ∧ P a')); [|naive_solver].
+    apply singleton_updateP', (iso_cmra_updateP' inG_fold).
+    { apply inG_unfold_fold. }
+    { apply (cmra_morphism_op _). }
+    { apply inG_unfold_validN. }
+    by apply cmra_transport_updateP'.
+  - apply exist_elim=> m; apply pure_elim_l=> -[a' [-> HP]].
+    rewrite -(exist_intro a'). rewrite -persistent_and_sep.
+    by apply and_intro; [apply pure_intro|].
+Qed.
+
+Lemma own_update γ a a' : a ~~> a' → own γ a ⊢ |==> own γ a'.
+Proof.
+  intros. iIntros "?".
+  iMod (own_updateP (a' =.) with "[$]") as (a'') "[-> $]".
+  { by apply cmra_update_updateP. }
+  done.
+Qed.
+Lemma own_update_2 γ a1 a2 a' :
+  a1 ⋅ a2 ~~> a' → own γ a1 -∗ own γ a2 ==∗ own γ a'.
+Proof. intros. apply entails_wand, wand_intro_r. rewrite -own_op. by iApply own_update. Qed.
+Lemma own_update_3 γ a1 a2 a3 a' :
+  a1 ⋅ a2 ⋅ a3 ~~> a' → own γ a1 -∗ own γ a2 -∗ own γ a3 ==∗ own γ a'.
+Proof. intros. apply entails_wand. do 2 apply wand_intro_r. rewrite -!own_op. by iApply own_update. Qed.
+End global.
+
+Global Arguments own_valid {_ _} [_] _ _.
+Global Arguments own_valid_2 {_ _} [_] _ _ _.
+Global Arguments own_valid_3 {_ _} [_] _ _ _ _.
+Global Arguments own_valid_l {_ _} [_] _ _.
+Global Arguments own_valid_r {_ _} [_] _ _.
+Global Arguments own_updateP {_ _} [_] _ _ _ _.
+Global Arguments own_update {_ _} [_] _ _ _ _.
+Global Arguments own_update_2 {_ _} [_] _ _ _ _ _.
+Global Arguments own_update_3 {_ _} [_] _ _ _ _ _ _.
+
+Lemma own_unit A `{i : !inG Σ (A:ucmra)} γ : ⊢ |==> own γ (ε:A).
+Proof.
+  rewrite /bi_emp_valid (ownM_unit emp) !own_eq /own_def.
+  apply bupd_ownM_update, discrete_fun_singleton_update_empty.
+  apply (alloc_unit_singleton_update (inG_unfold (cmra_transport inG_prf ε))).
+  - apply (cmra_morphism_valid _), cmra_transport_valid, ucmra_unit_valid.
+  - intros x. rewrite -(inG_unfold_fold x) -(cmra_morphism_op inG_unfold).
+    f_equiv. generalize (inG_fold x)=> x'.
+    destruct inG_prf=> /=. by rewrite left_id.
+  - done.
+Qed.
+-/
+
+
 
 end iOwn
 end Iris
